Simple_Clause_Learning/Termination.thy
@@ -449,29 +449,27 @@ next
           ground_prop: "is_ground_cls (add_mset K D \<cdot> \<gamma>\<^sub>D)"
           unfolding resolveI(1,2) \<open>\<Gamma> = trail_propagate \<Gamma>' K D \<gamma>\<^sub>D\<close>
           by (simp_all add: ground_closures_def propagate_lit_def)
+        hence
+          "\<forall>L\<in>#add_mset L C. L \<cdot>l \<rho>\<^sub>C \<cdot>l \<gamma> = L \<cdot>l \<gamma>\<^sub>C"
+          "\<forall>K\<in>#add_mset K D. K \<cdot>l \<rho>\<^sub>D \<cdot>l \<gamma> = K \<cdot>l \<gamma>\<^sub>D"
+          using resolveI merge_of_renamed_groundings by metis+
 
-        let ?\<gamma>\<^sub>D' = "restrict_subst_domain (vars_cls (add_mset K D)) \<gamma>\<^sub>D"
-
-        have "K \<cdot>l ?\<gamma>\<^sub>D' = K \<cdot>l \<gamma>\<^sub>D" and "D \<cdot> ?\<gamma>\<^sub>D' = D \<cdot> \<gamma>\<^sub>D"
-          by (simp_all add: subst_lit_restrict_subst_domain subst_cls_restrict_subst_domain)
-        hence "K \<cdot>l ?\<gamma>\<^sub>D' = - (L \<cdot>l \<gamma>\<^sub>C)" and ground_prop': "is_ground_cls (add_mset K D \<cdot> ?\<gamma>\<^sub>D')"
-          using \<open>K \<cdot>l \<gamma>\<^sub>D = - (L \<cdot>l \<gamma>\<^sub>C)\<close> ground_prop by simp_all
-
-        have dom_\<gamma>\<^sub>D': "subst_domain ?\<gamma>\<^sub>D' \<subseteq> vars_cls (add_mset K D)"
-          by simp
-
-        let ?\<gamma> = "rename_subst_domain \<rho>\<^sub>D ?\<gamma>\<^sub>D' \<odot> rename_subst_domain \<rho>\<^sub>C \<gamma>\<^sub>C"
-        have
-          "L \<cdot>l \<rho>\<^sub>C \<cdot>l ?\<gamma> = L \<cdot>l \<gamma>\<^sub>C" and
-          "C \<cdot> \<rho>\<^sub>C \<cdot> ?\<gamma> = C \<cdot> \<gamma>\<^sub>C" and
-          "K \<cdot>l \<rho>\<^sub>D \<cdot>l ?\<gamma> = K \<cdot>l \<gamma>\<^sub>D" and
-          "D \<cdot> \<rho>\<^sub>D \<cdot> ?\<gamma> = D \<cdot> \<gamma>\<^sub>D" and
-          "\<mu> \<odot> ?\<gamma> = ?\<gamma>"
-          using renamed_comp_renamed_simp[OF \<open>K \<cdot>l ?\<gamma>\<^sub>D' = - (L \<cdot>l \<gamma>\<^sub>C)\<close> ground_conf
-            ground_prop' dom_\<gamma>\<^sub>D' \<open>is_renaming \<rho>\<^sub>C\<close> \<open>is_renaming \<rho>\<^sub>D\<close>
-            \<open>vars_cls (add_mset L C \<cdot> \<rho>\<^sub>C) \<inter> vars_cls (add_mset K D \<cdot> \<rho>\<^sub>D) = {}\<close>]
-            \<open>is_imgu \<mu> {{atm_of L \<cdot>a \<rho>\<^sub>C, atm_of K \<cdot>a \<rho>\<^sub>D}}\<close> \<open>K \<cdot>l ?\<gamma>\<^sub>D' = K \<cdot>l \<gamma>\<^sub>D\<close> \<open>D \<cdot> ?\<gamma>\<^sub>D' = D \<cdot> \<gamma>\<^sub>D\<close>
-          by simp_all
+        have "atm_of L \<cdot>a \<rho>\<^sub>C \<cdot>a \<gamma> = atm_of K \<cdot>a \<rho>\<^sub>D \<cdot>a \<gamma>"
+          using \<open>K \<cdot>l \<gamma>\<^sub>D = - (L \<cdot>l \<gamma>\<^sub>C)\<close>
+            \<open>\<forall>L\<in>#add_mset L C. L \<cdot>l \<rho>\<^sub>C \<cdot>l \<gamma> = L \<cdot>l \<gamma>\<^sub>C\<close>[rule_format, of L, simplified]
+            \<open>\<forall>K\<in>#add_mset K D. K \<cdot>l \<rho>\<^sub>D \<cdot>l \<gamma> = K \<cdot>l \<gamma>\<^sub>D\<close>[rule_format, of K, simplified]
+          by (metis atm_of_eq_uminus_if_lit_eq atm_of_subst_lit)
+        hence "is_unifiers \<gamma> {{atm_of L \<cdot>a \<rho>\<^sub>C, atm_of K \<cdot>a \<rho>\<^sub>D}}"
+          by (simp add: is_unifiers_def is_unifier_alt)
+        hence "\<mu> \<odot> \<gamma> = \<gamma>"
+          using \<open>is_imgu \<mu> {{atm_of L \<cdot>a \<rho>\<^sub>C, atm_of K \<cdot>a \<rho>\<^sub>D}}\<close>
+          by (auto simp: is_imgu_def)
+        hence "C \<cdot> \<rho>\<^sub>C \<cdot> \<mu> \<cdot> \<gamma> = C \<cdot> \<gamma>\<^sub>C" and "D \<cdot> \<rho>\<^sub>D \<cdot> \<mu> \<cdot> \<gamma> = D \<cdot> \<gamma>\<^sub>D"
+          using \<open>\<forall>L\<in>#add_mset L C. L \<cdot>l \<rho>\<^sub>C \<cdot>l \<gamma> = L \<cdot>l \<gamma>\<^sub>C\<close> \<open>\<forall>K\<in>#add_mset K D. K \<cdot>l \<rho>\<^sub>D \<cdot>l \<gamma> = K \<cdot>l \<gamma>\<^sub>D\<close>
+          by (metis insert_iff same_on_lits_clause set_mset_add_mset_insert subst_cls_comp_subst
+              subst_lit_comp_subst)+
+        hence "(C \<cdot> \<rho>\<^sub>C + D \<cdot> \<rho>\<^sub>D) \<cdot> \<mu> \<cdot> \<gamma> = C \<cdot> \<gamma>\<^sub>C + D \<cdot> \<gamma>\<^sub>D"
+          by (metis subst_cls_comp_subst subst_cls_union)
 
         have "L \<cdot>l \<gamma>\<^sub>C \<notin># D \<cdot> \<gamma>\<^sub>D"
           using \<open>trail_resolved_lits_pol S\<close> \<open>K \<cdot>l \<gamma>\<^sub>D = - (L \<cdot>l \<gamma>\<^sub>C)\<close>
@@ -497,9 +495,7 @@ next
         thus ?thesis
           unfolding lex_prodp_def resolveI(1,2)
           unfolding \<M>_def state_proj_simp option.case prod.case prod.sel
-          unfolding \<open>\<gamma> = ?\<gamma>\<close>
-          unfolding subst_cls_comp_subst[symmetric] \<open>\<mu> \<odot> ?\<gamma> = ?\<gamma>\<close>
-          unfolding subst_cls_union \<open>C \<cdot> \<rho>\<^sub>C \<cdot> ?\<gamma> = C \<cdot> \<gamma>\<^sub>C\<close> \<open>D \<cdot> \<rho>\<^sub>D \<cdot> ?\<gamma> = D \<cdot> \<gamma>\<^sub>D\<close>
+          unfolding \<open>(C \<cdot> \<rho>\<^sub>C + D \<cdot> \<rho>\<^sub>D) \<cdot> \<mu> \<cdot> \<gamma> = C \<cdot> \<gamma>\<^sub>C + D \<cdot> \<gamma>\<^sub>D\<close>
           by simp
       qed
     qed
